examples/invariants/DY.Example.Invariants.Uniqueness.Next.fst
@@ -1,0 +1,147 @@
+module DY.Example.Invariants.Uniqueness.Next
+
+open Comparse
+open DY.Core
+module L = DY.Core.Label
+module Lib = DY.Lib
+module List = FStar.List.Tot.Base
+module Trace = DY.Core.Trace.Type
+
+open DY.Example.Invariants.Uniqueness
+
+#set-options "--fuel 1 --ifuel 1"
+
+
+#push-options "--fuel 2 --z3rlimit 20 --z3cliopt 'smt.qi.eager_threshold=20'"
+val state_same_idn_full_state_pred:
+  tr:trace -> p:principal -> sid:state_id 
+  -> old_cont:state_raw -> new_cont:state_raw
+  -> Lemma
+    (requires (
+         trace_invariant tr
+       /\ has_state_for tr p sid
+       /\ (let old_cont = access_state tr p sid in           
+            Some? (parse p_state old_cont )
+          /\ Some? (parse p_state new_cont )
+          /\ (let Some old_st = parse p_state old_cont in
+             let Some new_st = parse p_state new_cont in
+             old_st.idn = new_st.idn
+            )
+         )
+    ))
+    (ensures
+       full_state_pred tr (access_full_state tr p) p sid new_cont
+    )
+let state_same_idn_full_state_pred tr p sid old_cont new_cont =
+  let old_cont = access_state tr p sid in
+  let old_entry = (SetState p sid old_cont) in
+  let Some (S the_idn the_ctr) = parse p_state new_cont in
+
+  full_state_pred_forall_session_intro (access_full_state tr p) sid
+  (fun sid_i sess_i ->
+    let Snoc _ last_i = sess_i in
+         match parse p_state last_i with
+         | None -> True
+         | Some last_i -> last_i.idn <> the_idn
+  )
+  (fun sid_i sess_i ->
+     let Snoc _ last_i_b = sess_i in
+     match parse p_state last_i_b with
+     | None -> ()
+     | Some last_i -> (
+     full_state_mem_get_session_get_state_forall p tr;
+         let tr_after_old = tr `suffix_after_event` old_entry in
+         let last_i_entry = SetState p sid_i last_i_b in
+         let tr_after_last_i = tr `suffix_after_event` last_i_entry in
+         if tr_after_old `has_suffix` tr_after_last_i
+           then ( // last_i after oldst on tr
+             //admit();
+             assert(no_set_state_entry_for p sid tr_after_last_i);
+             let tr_before_last_i = tr `prefix_before_event` last_i_entry in
+             suff_after_before_event_is_suff_at_event tr last_i_entry;
+             no_set_state_entry_for_concat p sid (Snoc Nil last_i_entry) tr_after_last_i;
+             get_state_same p sid tr_before_last_i tr;
+             assert(old_cont = access_state tr_before_last_i p sid);
+             assert(global_state_pred tr_before_last_i p sid_i last_i_b);
+             get_state_appears_in_full_state tr_before_last_i p sid
+           )
+           else ( // oldst after last_i on tr
+             //admit();
+             suffixes tr tr_after_last_i tr_after_old;
+             assert(tr_after_last_i `has_suffix` tr_after_old);
+
+             get_state_no_set_state_for_on_suffix_after_event tr p sid_i;
+             no_set_state_entry_for_on_suffix tr_after_last_i tr_after_old p sid_i;
+             let tr_before_old = tr `prefix_before_event` old_entry in                               
+             suff_after_before_event_is_suff_at_event tr old_entry;
+             no_set_state_entry_for_concat p sid_i (Snoc Nil old_entry) tr_after_old;
+             get_state_same p sid_i tr_before_old tr;
+             let state_i_before_old = access_state tr_before_old p sid_i in
+             assert(state_i_before_old = last_i_b);
+             assert(global_state_pred tr_before_old p sid old_cont);
+             get_state_appears_in_full_state tr_before_old p sid_i  
+           )
+     )
+  )
+#pop-options
+
+#push-options "--z3rlimit 50 --z3cliopt 'smt.qi.eager_threshold=50'"
+val next_invariant: tr:trace -> p:principal -> sid:state_id ->
+  Lemma 
+    (requires trace_invariant tr)
+    (ensures  (
+      let (_,tr_out) = next p sid tr in
+      trace_invariant tr_out
+      )
+    )
+let next_invariant tr p sid = 
+  match get_state p sid tr with
+  | (None, _) -> ()
+  | (Some oldst_b, _) -> (
+      match parse p_state oldst_b with
+      | None -> ()
+      | Some (S idn c) -> (          
+          let msg = M p in
+          let msg_b = serialize message msg in
+          let (_, tr_after_msg) = send_msg msg_b tr in
+          serialize_wf_lemma message (is_publishable tr) msg;
+
+          let (_, tr_after_rand) = mk_rand NoUsage public 7 tr_after_msg in
+
+          let next_state = S idn (c+1) in
+          let next_state_b = serialize p_state next_state in
+          let (_,tr_after_next_state) = set_state p sid next_state_b tr_after_rand in
+          
+
+          serialize_wf_lemma p_state (is_knowable_by (principal_state_label p sid) tr_after_rand) next_state;
+
+          get_state_same p sid tr tr_after_msg;
+          get_state_same p sid tr_after_msg tr_after_rand;
+
+          state_same_idn_full_state_pred tr_after_rand p sid oldst_b (serialize p_state (S idn (c+1)));
+
+
+          let ev = E p in
+          let ev_b = serialize p_event ev in
+          let (_, tr_after_event) = trigger_event p "P" ev_b tr_after_next_state in
+
+          let other_sid = {the_id = sid.the_id + 1} in
+          match get_state p other_sid tr_after_event with
+          | (None, _ ) -> ()
+          | (Some ost_b, _) -> begin
+            match parse p_state ost_b with
+            | None -> ()
+            | Some (S other_idn other_c) ->
+               let other_state = S other_idn (other_c + 1) in
+               let other_state_b = serialize p_state other_state in
+               let (_, tr_after_other_session) = set_state p other_sid other_state_b tr_after_event in
+               
+               parse_wf_lemma #bytes p_state #_ (is_knowable_by (principal_state_label p other_sid) tr_after_event) ost_b;
+               serialize_wf_lemma p_state (is_knowable_by (principal_state_label p other_sid) tr_after_event) other_state;
+
+               state_same_idn_full_state_pred tr_after_event p other_sid ost_b other_state_b
+            end
+
+)
+    )
+#pop-options
